---
title: "Untitled"
author: "Caroline Ring"
date: "2023-05-10"
output: html_document
---

```{r setup, include=FALSE}
knitr::opts_chunk$set(echo = TRUE)
```

# MSE for individual observations

$$ \textrm{MSE} = \frac{1}{N} \sum_{i=1}^G \sum_{j=1}^{N_i} \left( y_{ij} - \mu_i \right)^2 $$
Expand the summand

$$ \textrm{MSE} = \frac{1}{N} \sum_{i=1}^G \sum_{j=1}^{N_i}  y_{ij}^2 - 2 y_{ij}\mu_i   + \mu_i^2 $$
Break appart the inner summation


$$ \textrm{MSE} = \frac{1}{N} \sum_{i=1}^G \left(
\sum_{j=1}^{N_i}  y_{ij}^2 -
2\mu_i \sum_{j=1}^{N_i} y_{ij}  +
N_i \mu_i^2 \right) $$



The definition of the sample variance is

$$ s_i^2 = \frac{1}{N_i - 1} \sum_{j=1}^{N_i} \left( y_{ij} - \bar{y}_{i} \right)^2 $$
which becomes

$$ s_i^2 = \frac{1}{N_i - 1} \sum_{j=1}^{N_i} \left( y_{ij}^2  - 2 y_{ij} \bar{y}_{i} + \bar{y}_{i}^2 \right) $$
which becomes

$$ s_i^2 = \frac{1}{N_i - 1} \left( \sum_{j=1}^{N_i} y_{ij}^2  - 2 \bar{y}_{i} \sum_{j=1}^{N_i} y_{ij}  + N_i \bar{y}_{i}^2 \right) $$
and using the definition of the sample mean,

$$ \bar{y}_i = \frac{1}{N_i} \sum_{j=1}^{N_i} y_{ij} $$

which means that

$$ \sum_{j=1}^{N_i} y_{ij} = N_i \bar{y}_i $$
then we can write the sample variance as

$$ s_i^2 = \frac{1}{N_i - 1} \left( \sum_{j=1}^{N_i} y_{ij}^2  - 2 N_i \bar{y}_i^2  + N_i \bar{y}_{i}^2 \right) $$

which simplifies to

$$ s_i^2 = \frac{1}{N_i - 1} \left( \sum_{j=1}^{N_i} y_{ij}^2  -  N_i \bar{y}_i^2  \right) $$
which means that

$$ \sum_{j=1}^{N_i} y_{ij}^2 = (N_i - 1) s_i^2 + N_i \bar{y}_i^2 $$

which we can substitute back into the equation for the MSE

$$ \textrm{MSE} = \frac{1}{N} \sum_{i=1}^G \left(
(N_i - 1) s_i^2 + N_i \bar{y}_i^2 -
2\mu_i N_i \bar{y}_i  +
N_i \mu_i^2 \right) $$
